<?xml version="1.0" encoding="UTF-8" standalone="no"?>
<!--
============================
RDFS Encoding of CRMtex v1.0 
============================

Created by Francesca Murano and Achille Felicetti on February 03, 2020

Encoding Rules:

1. The RDF spelling rules do not allow blanks. Hence we have replaced them by underscores.
   The blank between the concept identifier and concept name is replaced by underscore too.
   For instance "TX1_Written_Text" or "TXP1_used_writing_system".

2. RDF does not allow to instantiate properties beginning from a range value.
   Therefore, each CRMtex property is represented as two RDFS properties.
   For instance "TXP5 wrote (was written by)" is represented as:
   "TXP5_wrote" for the domain to range direction and "TXP5_was_written_by" for the range to domain direction.

3. Scope notes are represented as <rdf:comment> elements.

4. Any other differences in labels, scope notes  and semantic relationships of this encoding 
   to the authoritative definition of the FRBRoo v2.4 (November 2015) are not intended transfer errors. 
   The authors appreciate your feed-back on such errors.

-->
<rdf:RDF xmlns:rdf="http://www.w3.org/1999/02/22-rdf-syntax-ns#" xmlns:rdfs="http://www.w3.org/2000/01/rdf-schema#" xml:lang="en" xml:base="http://www.cidoc-crm.org/cidoc-crm/crmtex/">
	
	<rdfs:Class rdf:about="TX1_Written_Text">
		<rdfs:label xml:lang="en">TX1 Written Text</rdfs:label>
		<rdfs:comment>
			This class comprises visible set of symbols (glyphs or graphs) intentionally traced (i.e. “written”) on some kind of physical support by using specific techniques and having semiotic significance and the purpose of conveying a message towards a given addressee or group of addressees.
		</rdfs:comment>
		<rdfs:subClassOf rdf:resource="http://www.cidoc-crm.org/cidoc-crm/E25_Man-Made_Feature"/>
	</rdfs:Class>
	
	<rdfs:Class rdf:about="TX2_Writing">
		<rdfs:label xml:lang="en">TX2 Writing</rdfs:label>
		<rdfs:comment>
			Subclass of FRBR F28 Expression Creation indicating the activity of physically creating a text, using various techniques (painting, sculpture, etc.) and by means of specific tools, on a given carrier in a non-mechanical way. 
		</rdfs:comment>
		<rdfs:subClassOf rdf:resource="http://iflastandards.info/ns/fr/frbr/frbroo/F28_Expression_Creation"/>
	</rdfs:Class>

	<rdfs:Class rdf:about="TX3_Writing_System">
		<rdfs:label xml:lang="en">TX3 Writing System</rdfs:label>
		<rdfs:comment>
			Subclass of E29 Design or Procedure refers to a conventional system consisting of a set of signs (graphemes, TX8) used to codify a natural language, by means of specific rules in the combination and phonological value assignment of the chosen graphemes. As each code, a writing systems requires shared understanding between writers and readers allowing the transmission of the message. It is used to produce a TX1 Written Text during a TX2 Writing event. 
		</rdfs:comment>
		<rdfs:subClassOf rdf:resource="http://www.cidoc-crm.org/cidoc-crm/E29_Design_or_Procedure"/>
	</rdfs:Class>

	<rdfs:Class rdf:about="TX4_Writing_Field">
		<rdfs:label xml:lang="en">TX4 Writing Field</rdfs:label>
		<rdfs:comment>
			Subclass of E25 Man-Made Feature, it is the portion of the physical carrier arranged and usually reserved and delimited for the purpose of accommodating a written text, highlighting and isolating it from the other parts of the object to which it belongs, enhancing and guaranteeing its readability. This entity is paramount specially in epigraphy, in which a specific element called “epigraphic field” has been defined by the discipline itself. Its importance is also evident in papyrology and codicology, where a clear distinction between area(s) containing the written text and empty parts of the support (margins, intercolumnia, etc.) is significant for the definition of styles and periods of the document.  
		</rdfs:comment>
		<rdfs:subClassOf rdf:resource="http://www.cidoc-crm.org/cidoc-crm/E25_Man-Made_Feature"/>
	</rdfs:Class>

	<rdfs:Class rdf:about="TX5_Reading">
		<rdfs:label xml:lang="en">TX5 Reading</rdfs:label>
		<rdfs:comment>
		  Subclass of the S4 Observation, referring to the semiotic procedure of decoding (and therefore understanding) a written text. This procedure can be carried out for scientific purposes, in order to analyse and study the text according to different disciplinary perspectives. The reading activity, thus, is intended as a specific observation (S4) in which the decoding of the signs is performed, i.e. the linguistic value is recognised and the message is understood. Cases in which decoding does not happen (e.g., the observer is able to describe the signs but not to assign a specific linguist value to them), the S4 class could be used as it is. For study purposes, the reading procedure requires a scientific autoptic examination of the text as preparatory action for the study. An autoptic examination consists of an accurate analysis of the surface and the signs and prescribes the use of specific tools and procedures, for establishing as faithfully as possible the exact value of each sign drawn on the physical feature. 
		</rdfs:comment>
		<rdfs:subClassOf rdf:resource="http://www.ics.forth.gr/isl/CRMext/CRMsci.rdfs/S4_Observation"/>
	</rdfs:Class>

	<rdfs:Class rdf:about="TX6_Transcription">
		<rdfs:label xml:lang="en">TX6 Transcription</rdfs:label>
		<rdfs:comment>
		  Subclass of E7 Activity, referring to the activity of re-writing the text conducted by an editor. This operation could involve a writing system (TX3) different from that of the original text, implying a transposition of the sounds of a language from a writing system to another one (e.g., Latin letters to render a Mycenaean text). For scientific purposes, this operation often consists in a ‘transliteration’, because it implies a 1:1 relation between the signs of the two writing systems. The P16 used specific object (was used for) property can be used to specify the role of the original graphemes during the commuting operations. 
		</rdfs:comment>
		<rdfs:subClassOf rdf:resource="http://www.cidoc-crm.org/cidoc-crm/E7_Activity"/>
	</rdfs:Class>

	<rdfs:Class rdf:about="TX7_Written_Text_Segment">
		<rdfs:label xml:lang="en">TX7 Written Text Segment</rdfs:label>
		<rdfs:comment>
		  Subclass of TX1 Written Text intended to identify portions of text considered to be of particular significance by scholars, as witnesses of a certain meaning or bearers of a particular phenomenon relevant to the investigation, study and understanding of the ancient text. Examples of such text portions are: columns, fragments, sections, paragraphs, as well as single words or letters, or other components of the written text. To each of these entities can be associated a single production event (TX2) or destruction event (E6), as in the case of letters or words damaged or worn by atmospheric agents or human interventions, as well as specific conditions (E3) for documenting its status during the observation process (S4). The relationship between a written text (TX1) and its components is documented through the TXP4 has segment property. 
		</rdfs:comment>
		<rdfs:subClassOf rdf:resource="TX1_Written_Text"/>
	</rdfs:Class>

	<rdfs:Class rdf:about="TX8_Grapheme">
		<rdfs:label xml:lang="en">TX8 Grapheme</rdfs:label>
		<rdfs:comment>
		  Subclass of E90 Symbolic Object used to represent the abstract units with distinctive value in a given writing system. A grapheme is a character or sequence of characters that functions as a distinct unit within an orthography. It may be a single character, a multigraph, or a diacritic, but in all cases graphemes are defined in relation to the particular orthography. Most graphemes represent a single phoneme, but some represent a sequence of phonemes. For instance, the character sequence ‹ch› is often used to represent the phoneme /tʃ/ in English, while the single letter ‹x› usually represents the phoneme sequence /ks/. In a highly phonemic writing system, there is a close correspondence between graphemes and phonemes. English (written with Latin script) is an example of a writing system that is not highly phonemic, and therefore the mappings between graphemes and phonemes are more complex. Graphemes are often written enclosed in angle brackets (‹›).
		</rdfs:comment>
		<rdfs:subClassOf rdf:resource="http://www.cidoc-crm.org/cidoc-crm/E90_Symbolic_Object"/>
	</rdfs:Class>

	<rdfs:Class rdf:about="TX9_Glyph">
		<rdfs:label xml:lang="en">TX9 Glyph</rdfs:label>
		<rdfs:comment>
		  Subclass of E25 Man-Made Feature intended to represent the concrete manifestation of single signs traced by the writer while codifying a linguistic expression. Glyphs are typically observed by the scholar during a reading activity (TX5) carried out to decode and recognise the graphemes (TX8) they represent.
		</rdfs:comment>
		<rdfs:subClassOf rdf:resource="http://www.cidoc-crm.org/cidoc-crm/E25_Man-Made_Feature"/>
	</rdfs:Class>

	<rdfs:Class rdf:about="TX10_Style">
		<rdfs:label xml:lang="en">TX10 Style</rdfs:label>
		<rdfs:comment>
		  SSubclass of E29 Design or Procedure that describes styles and variations of texts, including local script styles (Carolingian minuscule) and individual scribal hands. It includes: the general appearance of the script, in terms of general design, aspects related to a bilinear system (i.e. upper and lowercases), measures (i.e. large, medium or small), shape and number of strokes forming a character, its order and direction. A style includes also information about ductus (the direction the text is written), ligatures and nexi (i.e. the connection between characters obtained tracing them without detaching the writing instrument from the support and using one or more strokes in common), and the writing angle (i.e. the position the writing instrument is located with respect to the support). The style corresponds to fonts and their variations in modern printing process.
		</rdfs:comment>
		<rdfs:subClassOf rdf:resource="http://www.cidoc-crm.org/cidoc-crm/E29_Design_or_Procedure"/>
	</rdfs:Class>

<!-- ======== CRMtex Properties ======== -->

<!-- TXP1 used writing system (writing system used for) -->
	<rdf:Property rdf:about="TXP1_used_writing_system">
		<rdfs:label xml:lang="en">TXP1 used writing system</rdfs:label>
		<rdfs:comment>
		 This property is intended to identify the specific instance of TX3 Writing System employed during the writing event that led to the creation of a TX1 Written Text. 
		</rdfs:comment>
		<rdfs:domain rdf:resource="TX2_Writing"/>
		<rdfs:range rdf:resource="TX3_Writing_System"/>
		<rdfs:subPropertyOf rdf:resource="http://www.cidoc-crm.org/cidoc-crm/P33_used_specific_technique"/>
	</rdf:Property>

	<rdf:Property rdf:about="TXP1i_writing_system_used_for">
		<rdfs:label xml:lang="en">TXP1i writing system used for</rdfs:label>
		<rdfs:comment>
		 This property is intended to identify the specific instance of TX3 Writing System employed during the writing event that led to the creation of a TX1 Written Text. 
		</rdfs:comment>
		<rdfs:domain rdf:resource="TX3_Writing_System"/>
		<rdfs:range rdf:resource="TX2_Writing"/>
		<rdfs:subPropertyOf rdf:resource="http://www.cidoc-crm.org/cidoc-crm/P33i_was_used_by"/>
	</rdf:Property>

<!-- TXP2 includes (is included within) -->
	<rdf:Property rdf:about="TXP2_includes">
		<rdfs:label xml:lang="en">TXP2 includes</rdfs:label>
		<rdfs:comment>
		  This property is intended to describe the relation existing between a TX1 Written Text and the TX4 Writing Field, specifically created to accommodate the text, within which it is inscribed. This relation becomes quite relevant in the very frequent case where more than a single text is found on different areas of a specific support.
		</rdfs:comment>
		<rdfs:domain rdf:resource="TX4_Writing_Field"/>
		<rdfs:range rdf:resource="TX1_Written_Text"/>
		<rdfs:subPropertyOf rdf:resource="http://www.cidoc-crm.org/cidoc-crm/P56_bears_feature"/>
	</rdf:Property>

	<rdf:Property rdf:about="TXP2i_is_included_within">
		<rdfs:label xml:lang="en">TXP2i is included within</rdfs:label>
		<rdfs:comment>
		  This property is intended to describe the relation existing between a TX1 Written Text and the TX4 Writing Field, specifically created to accommodate the text, within which it is inscribed. This relation becomes quite relevant in the very frequent case where more than a single text is found on different areas of a specific support.
		</rdfs:comment>
		<rdfs:domain rdf:resource="TX1_Written_Text"/>
		<rdfs:range rdf:resource="TX4_Writing_Field"/>
		<rdfs:subPropertyOf rdf:resource="http://www.cidoc-crm.org/cidoc-crm/P56i_is_found_on"/>
	</rdf:Property>

<!-- TXP3 rendered (is rendered by) -->
	<rdf:Property rdf:about="TXP3_rendered">
		<rdfs:label xml:lang="en">TXP3 rendered</rdfs:label>
		<rdfs:comment>
		  This property is intended to emphasize the close connection for scientific purposes between the TX5 Reading and TX6 Transcription activities, by outlining, in particular, the accurate observation required by scholars in order to perform a valid transcription of a given text.
		</rdfs:comment>
		<rdfs:domain rdf:resource="TX6_Transcription"/>
		<rdfs:range rdf:resource="TX5_Reading"/>
		<rdfs:subPropertyOf rdf:resource="http://www.cidoc-crm.org/cidoc-crm/P20_had_specific_purpose"/>
	</rdf:Property>

	<rdf:Property rdf:about="TXP3i_is_rendered_by">
		<rdfs:label xml:lang="en">TXP3i is rendered by</rdfs:label>
		<rdfs:comment>
		  This property is intended to emphasize the close connection for scientific purposes between the TX5 Reading and TX6 Transcription activities, by outlining, in particular, the accurate observation required by scholars in order to perform a valid transcription of a given text.
		</rdfs:comment>
		<rdfs:domain rdf:resource="TX5_Reading"/>
		<rdfs:range rdf:resource="TX6_Transcription"/>
		<rdfs:subPropertyOf rdf:resource="http://www.cidoc-crm.org/cidoc-crm/P20i_was_purpose_of"/>
	</rdf:Property>

<!-- TXP4 has segment (is segment of) -->
	<rdf:Property rdf:about="TXP4_has_segment">
		<rdfs:label xml:lang="en">TXP4 has segment</rdfs:label>
		<rdfs:comment>
		  This property is intended to correlate a text and the different parts of which a scholar can identify, such as: letters, words, lines, columns, pages, or any other scan that can be made by scholars because considered to have a particular relevance for the investigation of the text itself.
		</rdfs:comment>		
		<rdfs:domain rdf:resource="TX1_Written_Text"/>
		<rdfs:range rdf:resource="TX7_Written_Text_Segment"/>
		<rdfs:subPropertyOf rdf:resource="http://www.cidoc-crm.org/cidoc-crm/P46_is_composed_of"/>
	</rdf:Property>

	<rdf:Property rdf:about="TXP4i_is_segment_of">
		<rdfs:label xml:lang="en">TXP4i is segment of</rdfs:label>
		<rdfs:comment>
		  This property is intended to correlate a text and the different parts of which a scholar can identify, such as: letters, words, lines, columns, pages, or any other scan that can be made by scholars because considered to have a particular relevance for the investigation of the text itself.
		</rdfs:comment>	
		<rdfs:domain rdf:resource="TX7_Written_Text_Segment"/>
		<rdfs:range rdf:resource="TX1_Written_Text"/>
		<rdfs:subPropertyOf rdf:resource="http://www.cidoc-crm.org/cidoc-crm/P46i_forms_part_of"/>
	</rdf:Property>

<!-- TXP5 wrote (was written by) -->
	<rdf:Property rdf:about="TXP5_wrote">
		<rdfs:label xml:lang="en">TXP5 wrote</rdfs:label>
		<rdfs:comment>
		  This property is used to describe in detail the close relationship between a text and the writing event that led to its production.
		</rdfs:comment>
		<rdfs:domain rdf:resource="TX2_Writing"/>
		<rdfs:range rdf:resource="TX1_Written_Text"/>
		<rdfs:subPropertyOf rdf:resource="http://www.cidoc-crm.org/cidoc-crm/P108_has_produced"/>
	</rdf:Property>

	<rdf:Property rdf:about="TXP5i_was_written_by">
		<rdfs:label xml:lang="en">TXP5i was written by</rdfs:label>
		<rdfs:comment>
		  This property is used to describe in detail the close relationship between a text and the writing event that led to its production.
		</rdfs:comment>
		<rdfs:domain rdf:resource="TX1_Written_Text"/>
		<rdfs:range rdf:resource="TX2_Writing"/>
		<rdfs:subPropertyOf rdf:resource="http://www.cidoc-crm.org/cidoc-crm/P108i_was_produced_by"/>
	</rdf:Property>

<!-- TXP6 encodes (is encoding of) -->
	<rdf:Property rdf:about="TXP6_encodes">
		<rdfs:label xml:lang="en">TXP6 encodes</rdfs:label>
		<rdfs:comment>
		  This property is used to indicate the language encoded by the TX3 Writing System and used for writing, reading or rendering (i.e. transcribing) a TX1 Written Text. The specification of the language is fundamental for understanding the writing phenomena and the rules of the writing system used for the production or transcription of a specific text.
		</rdfs:comment>
		<rdfs:domain rdf:resource="TX3_Writing_System"/>
		<rdfs:range rdf:resource="http://www.cidoc-crm.org/cidoc-crm/E33_Linguistic_Object"/>
		<rdfs:subPropertyOf rdf:resource="http://www.cidoc-crm.org/cidoc-crm/P2_has_type"/>
	</rdf:Property>

	<rdf:Property rdf:about="TXP6i_is_encoding_of">
		<rdfs:label xml:lang="en">TXP6i is encoding of</rdfs:label>
		<rdfs:comment>
		  This property is used to indicate the language encoded by the TX3 Writing System and used for writing, reading or rendering (i.e. transcribing) a TX1 Written Text. The specification of the language is fundamental for understanding the writing phenomena and the rules of the writing system used for the production or transcription of a specific text.
		</rdfs:comment>
		<rdfs:domain rdf:resource="http://www.cidoc-crm.org/cidoc-crm/E33_Linguistic_Object"/>
		<rdfs:range rdf:resource="TX3_Writing_System"/>
		<rdfs:subPropertyOf rdf:resource="http://www.cidoc-crm.org/cidoc-crm/P2i_is_type_of"/>
	</rdf:Property>

<!-- TXP7 has item (is item of) -->
	<rdf:Property rdf:about="TXP7_has_item">
		<rdfs:label xml:lang="en">TXP7 has item</rdfs:label>
		<rdfs:comment>
		  This property is used to state the (conceptual) belonging of a TX8 Grapheme to a given TX3 Writing System.
		</rdfs:comment>
		<rdfs:domain rdf:resource="TX3_Writing_System"/>
		<rdfs:range rdf:resource="TX8_Grapheme"/>
		<rdfs:subPropertyOf rdf:resource="http://www.cidoc-crm.org/cidoc-crm/P106_is_composed_of"/>
	</rdf:Property>

	<rdf:Property rdf:about="TXP7i_is_item_of">
		<rdfs:label xml:lang="en">TXP7i is item of</rdfs:label>
		<rdfs:comment>
		  This property is used to state the (conceptual) belonging of a TX8 Grapheme to a given TX3 Writing System.
		</rdfs:comment>
		<rdfs:domain rdf:resource="TX8_Grapheme"/>
		<rdfs:range rdf:resource="TX3_Writing_System"/>
		<rdfs:subPropertyOf rdf:resource="http://www.cidoc-crm.org/cidoc-crm/P106i_forms_part_of"/>
	</rdf:Property>

<!-- TXP8 contains (is contained in) -->
	<rdf:Property rdf:about="TXP8_contains">
		<rdfs:label xml:lang="en">TXP8 contains</rdfs:label>
		<rdfs:comment>
		  This property is used to state the (physical) belonging of a TX9 Gliph to a given TX1 Written Text.
		</rdfs:comment>
		<rdfs:domain rdf:resource="TX1_Written_Text"/>
		<rdfs:range rdf:resource="TX9_Glyph"/>
		<rdfs:subPropertyOf rdf:resource="http://www.cidoc-crm.org/cidoc-crm/P46_is_composed_of"/>
	</rdf:Property>

	<rdf:Property rdf:about="TXP8i_is_contained_in">
		<rdfs:label xml:lang="en">TXP8i is contained in</rdfs:label>
		<rdfs:comment>
		  This property is used to state the (physical) belonging of a TX9 Gliph to a given TX1 Written Text.
		</rdfs:comment>
		<rdfs:domain rdf:resource="TX9_Glyph"/>
		<rdfs:range rdf:resource="TX1_Written_Text"/>
		<rdfs:subPropertyOf rdf:resource="http://www.cidoc-crm.org/cidoc-crm/P46i_forms_part_of"/>
	</rdf:Property>

<!-- TXP9 is encoded by (was used to encode) -->
	<rdf:Property rdf:about="TXP9_is_encoded_by">
		<rdfs:label xml:lang="en">TXP9 is encoded by</rdfs:label>
		<rdfs:comment>
		  This property has the purpose of directly associating a TX1 Written Text with the TX3 Writing System from which the signs used for its writing and therefore incorporated in the text have been taken. It is a shortcut of the more fully articulated path from TX1 Written Text, through TXP5 wrote (was written by), TX2 Writing, TXP1 used writing system (writing system used for) to TX3 Writing System.
		</rdfs:comment>
		<rdfs:domain rdf:resource="TX1_Written_Text"/>
		<rdfs:range rdf:resource="TX3_Writing_System"/>
	</rdf:Property>

	<rdf:Property rdf:about="TXP9i_was_used_to_encode">
		<rdfs:label xml:lang="en">TXP9i was used to encode</rdfs:label>
		<rdfs:comment>
		  This property has the purpose of directly associating a TX1 Written Text with the TX3 Writing System from which the signs used for its writing and therefore incorporated in the text have been taken. It is a shortcut of the more fully articulated path from TX1 Written Text, through TXP5 wrote (was written by), TX2 Writing, TXP1 used writing system (writing system used for) to TX3 Writing System.
		</rdfs:comment>
		<rdfs:domain rdf:resource="TX3_Writing_System"/>
		<rdfs:range rdf:resource="TX1_Written_Text"/>
	</rdf:Property>

<!-- TXP10 read (was read by) -->
	<rdf:Property rdf:about="TXP10_read">
		<rdfs:label xml:lang="en">TXP10 read</rdfs:label>
		<rdfs:comment>
		  This property links an instance of  TX1 Written Text with a TX5 Reading event carried out to investigate its intrinsic characteristics and to perform its decoding.
		</rdfs:comment>
		<rdfs:domain rdf:resource="TX5_Reading"/>
		<rdfs:range rdf:resource="TX1_Written_Text"/>
		<rdfs:subPropertyOf rdf:resource="http://www.ics.forth.gr/isl/CRMext/CRMsci.rdfs/O8_observed"/>
	</rdf:Property>

	<rdf:Property rdf:about="TXP10i_was_read_by">
		<rdfs:label xml:lang="en">TXP10i was read by</rdfs:label>
		<rdfs:comment>
		  This property links an instance of  TX1 Written Text with a TX5 Reading event carried out to investigate its intrinsic characteristics and to perform its decoding.
		</rdfs:comment>
		<rdfs:domain rdf:resource="TX1_Written_Text"/>
		<rdfs:range rdf:resource="TX5_Reading"/> <!-- http://www.ics.forth.gr/isl/CRMext/CRMsci.rdfs/S4_Observation -->
		<rdfs:subPropertyOf rdf:resource="http://www.ics.forth.gr/isl/CRMext/CRMsci.rdfs/O8i_was_observed_by"/>
	</rdf:Property>

<!-- TXP11 transcribed (was transcribed by) -->
	<rdf:Property rdf:about="TXP11_transcribed">
		<rdfs:label xml:lang="en">TXP11 transcribed</rdfs:label>
		<rdfs:comment>
		  This property highlights the specific way in which an activity of TX6 Transcription results in the rendering of the specific TX8 Grapheme(s) of which an instance of TX1 Written Text is composed.
		</rdfs:comment>
		<rdfs:domain rdf:resource="TX6_Transcription"/>
		<rdfs:range rdf:resource="TX8_Grapheme"/>
		<rdfs:subPropertyOf rdf:resource="http://www.cidoc-crm.org/cidoc-crm/P16_used_specific_object"/>
	</rdf:Property>

	<rdf:Property rdf:about="TXP11i_was_transcribed_by">
		<rdfs:label xml:lang="en">TXP11i was transcribed by</rdfs:label>
		<rdfs:comment>
		  This property highlights the specific way in which an activity of TX6 Transcription results in the rendering of the specific TX8 Grapheme(s) of which an instance of TX1 Written Text is composed.
		</rdfs:comment>
		<rdfs:domain rdf:resource="TX8_Grapheme"/>
		<rdfs:range rdf:resource="TX6_Transcription"/>
		<rdfs:subPropertyOf rdf:resource="http://www.cidoc-crm.org/cidoc-crm/P16i_was_used_for"/>
	</rdf:Property>



<!-- TXP12 has style (is style of) -->
	<rdf:Property rdf:about="TXP12_has_style">
		<rdfs:label xml:lang="en">TXP12 has style</rdfs:label>
		<rdfs:comment>
		  This property assigns information to a certain script in order to accurately determine the style used for the realization of the written text. The TPX12.1 has type property of TXP12 has style allows the nature of the style to be specified reading from domain to range, for example to record the ductus, orientation or the linear system of the text.
		</rdfs:comment>
		<rdfs:domain rdf:resource="TX1_Written_Text"/>
		<rdfs:range rdf:resource="TX10_Style"/>
		<rdfs:subPropertyOf rdf:resource="http://www.cidoc-crm.org/cidoc-crm/P33_used_specific_technique"/>
	</rdf:Property>

	<rdf:Property rdf:about="TXP12i_is_style_of)">
		<rdfs:label xml:lang="en">TXP12i is style of</rdfs:label>
		<rdfs:comment>
		  This property assigns information to a certain script in order to accurately determine the style used for the realization of the written text. The TPX12.1 has type property of TXP12 has style allows the nature of the style to be specified reading from domain to range, for example to record the ductus, orientation or the linear system of the text.
		</rdfs:comment>
		<rdfs:domain rdf:resource="TX10_Style"/>
		<rdfs:range rdf:resource="TX1_Written_Text"/>
		<rdfs:subPropertyOf rdf:resource="http://www.cidoc-crm.org/cidoc-crm/P33i_was_used_by"/>
	</rdf:Property>
	
</rdf:RDF>
